theories/zoo_saturn/mpsc_queue_3.v
@@ -529,7 +529,7 @@ Section mpsc_queue_3_G.
         iSplitR "HΦ". { iSteps. iExists back. iSteps. }
         iSteps.
 
-      + wp_cas as _ | []%(inj clist_to_val ClistClosed)%list_to_clist_open_not_closed'.
+      + wp_cas as _ | []%(inj clist_to_val ClstClosed)%list_to_clist_open_not_closed'.
         iSteps.
 
     - iMod "HΦ" as "(%vs & Hmodel & _ & HΦ)".
@@ -607,8 +607,8 @@ Section mpsc_queue_3_G.
 
         remember (back ++ [v]) as back' eqn:Hback.
         destruct back' as [| v' back']; first by eelim app_cons_not_nil.
-        wp_smart_apply (clst_rev_app_spec (v' :: back') ClistOpen with "[//]") as "_"; [done.. |].
-        rewrite clist_app_ClistOpen {}Hback reverse_snoc.
+        wp_smart_apply (clst_rev_app_spec (v' :: back') ClstOpen with "[//]") as "_"; [done.. |].
+        rewrite clist_app_ClstOpen {}Hback reverse_snoc.
         iSteps.
 
     - wp_store. wp_pures.
@@ -702,12 +702,12 @@ Section mpsc_queue_3_G.
     iModIntro. clear.
 
     iApply wp_match_clist_open. simpl.
-    wp_apply (clst_rev_app_spec _ ClistClosed with "[//]") as "_"; [done.. |].
+    wp_apply (clst_rev_app_spec _ ClstClosed with "[//]") as "_"; [done.. |].
     wp_load.
     wp_apply (clst_app_spec with "[//]") as "_"; [done.. |].
     wp_store.
 
-    iSteps. rewrite clist_app_ClistClosed. erewrite clist_app_closed => //.
+    iSteps. rewrite clist_app_ClstClosed. erewrite clist_app_closed => //.
   Qed.
   Lemma mpsc_queue_3_close_spec_closed t ι vs :
     {{{
